extraction/theories/OptimizeCorrectness.v
@@ -1,0 +1,1189 @@
+From ConCert.Extraction Require Import ExAst.
+From ConCert.Extraction Require Import ExTyping.
+From ConCert.Extraction Require Import Optimize.
+From Coq Require Import Arith.
+From Coq Require Import Bool.
+From Coq Require Import List.
+From Coq Require Import Psatz.
+From Equations Require Import Equations.
+From MetaCoq.Erasure Require Import EAstUtils.
+From MetaCoq.Erasure Require Import ECSubst.
+From MetaCoq.Erasure Require Import EInduction.
+From MetaCoq.Erasure Require Import ELiftSubst.
+From MetaCoq.Erasure Require Import EWcbvEval.
+From MetaCoq.Template Require Import utils.
+
+Import ListNotations.
+Set Equations Transparent.
+
+Import EAstUtils.
+Import Erasure.
+Import ExAst.
+
+(* We have our own environment which is different from MetaCoq's erased environment
+   (it includes more information and a different treatment of types).
+   To reconcile this, we map our environments to theirs, but the treatment of types
+   remains different. However, MetaCoq does not actually use information about types
+   for anything during evaluation, so we just filter them out. This is justified
+   by the following lemmas. *)
+Definition is_constant (decl : EAst.global_decl) : bool :=
+  match decl with
+  | EAst.ConstantDecl _ => true
+  | _ => false
+  end.
+
+Definition only_constants (Σ : EAst.global_context) : EAst.global_context :=
+  filter (is_constant ∘ snd) Σ.
+
+Lemma declared_constant_only_constants Σ kn decl :
+  ETyping.declared_constant Σ kn decl ->
+  ETyping.declared_constant (only_constants Σ) kn decl.
+Proof.
+  unfold ETyping.declared_constant.
+  intros lookup_decl.
+  induction Σ; [easy|].
+  destruct a as (kn' & decl').
+  cbn in *.
+  destruct (is_constant decl') eqn:isconst.
+  - cbn in *.
+    destruct (kername_eq_dec _ _) as [<-|?]; easy.
+  - apply IHΣ.
+    destruct (kername_eq_dec _ _).
+    + inversion lookup_decl; subst; easy.
+    + auto.
+Qed.
+
+Local Notation "Σ ⊢ s ▷ t" := (eval Σ s t) (at level 50, s, t at next level) : type_scope.
+
+Lemma eval_only_constants Σ s t :
+  Σ ⊢ s ▷ t ->
+  only_constants Σ ⊢ s ▷ t.
+Proof.
+  induction 1 using eval_evals_ind;
+    eauto using eval, declared_constant_only_constants.
+Qed.
+
+Definition trans_cst (cst : constant_body) : EAst.constant_body :=
+  {| EAst.cst_body := cst_body cst |}.
+
+Definition trans (Σ : global_env) : EAst.global_context :=
+  let map_decl kn (decl : global_decl) : list (kername * EAst.global_decl) :=
+      match decl with
+      | ConstantDecl cst => [(kn, EAst.ConstantDecl (trans_cst cst))]
+      | InductiveDecl _ => []
+      end in
+  flat_map (fun '(kn, decl) => map_decl kn decl) Σ.
+
+Lemma declared_constant_trans Σ kn cst :
+  declared_constant Σ kn cst ->
+  ETyping.declared_constant (trans Σ) kn (trans_cst cst).
+Proof.
+  unfold ETyping.declared_constant, declared_constant in *.
+  induction Σ; [easy|]; intros lookup.
+  cbn in *.
+  destruct a as (kn' & []).
+  - cbn in *.
+    unfold eq_kername in *.
+    destruct (kername_eq_dec kn kn') as [<-|].
+    + now inversion lookup; subst; clear lookup.
+    + now apply IHΣ.
+  - apply IHΣ.
+    unfold eq_kername in lookup.
+    now destruct (kername_eq_dec _ _).
+Qed.
+
+(*
+Section eta_correctness.
+Context (ctors : list (inductive * nat * nat)).
+Context (consts : list (kername * nat)).
+
+Notation eta_ctor := (eta_ctor ctors).
+Notation eta_const := (eta_const consts).
+Notation eta_expand_aux := (eta_expand_aux ctors consts).
+Notation eta_expand := (eta_expand ctors consts).
+
+Open Scope type.
+
+Lemma wfe_term_eta_single Σ t args n :
+  wfe_term Σ t ->
+  Forall (wfe_term Σ) args ->
+  wfe_term Σ (eta_single t args n).
+Proof.
+  intros wft wfall.
+  unfold eta_single.
+  induction (_ - _) at 3; [|easy].
+  cbn in *.
+  apply wfe_term_mkApps; [easy|].
+  apply Forall_app_inv.
+  - clear -wfall.
+    generalize args at 1; intros.
+    induction wfall; cbn in *; [easy|].
+    constructor; [|easy].
+    now apply wfe_term_lift.
+  - clear.
+    induction (seq _ _); [cbn; easy|].
+    rewrite rev_map_cons.
+    apply Forall_app_inv; [easy|].
+    constructor; easy.
+Qed.
+
+Lemma wfe_term_eta_ctor Σ ind i args :
+  wfe_term Σ (tConstruct ind i) ->
+  Forall (wfe_term Σ) args ->
+  wfe_term Σ (eta_ctor ind i args).
+Proof.
+  intros wft wfall.
+  unfold eta_ctor.
+  destruct (find _ _) as [((? & ?) & ?)|].
+  - now apply wfe_term_eta_single.
+  - now apply wfe_term_mkApps.
+Qed.
+
+Lemma wfe_term_eta_const Σ kn args :
+  wfe_term Σ (tConst kn) ->
+  Forall (wfe_term Σ) args ->
+  wfe_term Σ (eta_const kn args).
+Proof.
+  intros wft wfall.
+  unfold eta_const.
+  destruct (find _ _) as [((? & ?) & ?)|].
+  - now apply wfe_term_eta_single.
+  - now apply wfe_term_mkApps.
+Qed.
+
+Lemma wfe_term_eta_expand_aux Σ args t :
+  Forall (wfe_term Σ) args ->
+  wfe_term Σ t ->
+  wfe_term Σ (eta_expand_aux args t).
+Proof.
+  revert args.
+  induction t using term_forall_list_ind; intros args wfall wft; cbn in *; auto.
+  - now apply wfe_term_mkApps.
+  - now apply wfe_term_mkApps.
+  - now apply wfe_term_mkApps.
+  - apply wfe_term_mkApps; [|easy].
+    now induction H; cbn in *.
+  - now apply wfe_term_mkApps.
+  - apply wfe_term_mkApps; cbn; easy.
+  - apply IHt1; [|easy].
+    constructor; [|easy].
+    now apply IHt2.
+  - now apply wfe_term_eta_const.
+  - now apply wfe_term_eta_ctor.
+  - apply wfe_term_mkApps; [|easy].
+    cbn.
+    destruct p.
+    split; [easy|].
+    split; [easy|].
+    destruct wft as (_ & (_ & allwf)).
+    induction X; cbn in *; easy.
+  - now apply wfe_term_mkApps.
+  - apply wfe_term_mkApps; [|easy].
+    induction H; cbn in *; easy.
+  - apply wfe_term_mkApps; [|easy].
+    induction H; cbn in *; easy.
+Qed.
+
+Lemma wfe_term_eta_expand Σ t :
+  wfe_term Σ t ->
+  wfe_term Σ (eta_expand t).
+Proof. now apply wfe_term_eta_expand_aux. Qed.
+
+Lemma decompose_app_rec_app t acc acc' :
+  let (hd, args) := decompose_app_rec t acc in
+  decompose_app_rec t (acc ++ acc') = (hd, args ++ acc').
+Proof.
+  revert acc.
+  induction t using term_forall_list_ind; intros acc; try easy.
+  cbn.
+  specialize (IHt1 (t2 :: acc)).
+  now rewrite <- app_comm_cons in IHt1.
+Qed.
+
+Lemma eta_expand_aux_unfold t args :
+  eta_expand_aux args t =
+  match decompose_app t with
+  | (tConstruct ind c, args') => eta_ctor ind c (map (eta_expand_aux []) args' ++ args)
+  | (tConst kn, args') => eta_const kn (map (eta_expand_aux []) args' ++ args)
+  | (hd, args') => mkApps
+                     (map_subterms (eta_expand_aux []) hd)
+                     (map (eta_expand_aux []) args' ++ args)
+  end.
+Proof.
+  revert args.
+  induction t using term_forall_list_ind; intros args; cbn in *;
+    try easy.
+  rewrite IHt1.
+  unfold decompose_app.
+  pose proof (decompose_app_rec_app t1 [] [t2]).
+  destruct (decompose_app_rec t1 []) as [hd args'].
+  cbn in *.
+  rewrite H.
+  rewrite map_app.
+  cbn.
+  now rewrite <- app_assoc.
+Qed.
+
+Lemma eta_expand_unfold t :
+  eta_expand t =
+  match decompose_app t with
+  | (tConstruct ind c, args) => eta_ctor ind c (map eta_expand args)
+  | (tConst kn, args) => eta_const kn (map eta_expand args)
+  | (hd, args) => mkApps (map_subterms eta_expand hd) (map eta_expand args)
+  end.
+Proof.
+  unfold eta_expand at 1.
+  rewrite eta_expand_aux_unfold.
+  destruct (decompose_app _).
+  now rewrite app_nil_r.
+Qed.
+
+End eta_correctness.
+*)
+
+Section dearg_correctness.
+Context (ind_masks : list (kername * mib_masks)).
+Context (const_masks : list (kername * bitmask)).
+
+Fixpoint has_use (rel : nat) (t : term) : bool :=
+  match t with
+  | tRel i => i =? rel
+  | tEvar _ ts => fold_right orb false (map (has_use rel) ts)
+  | tLambda _ body => has_use (S rel) body
+  | tLetIn _ val body => has_use rel val || has_use (S rel) body
+  | tApp hd arg => has_use rel hd || has_use rel arg
+  | tCase _ _ brs => fold_right orb false (map (has_use rel ∘ snd) brs)
+  | tProj _ t => has_use rel t
+  | tFix defs _
+  | tCoFix defs _ => fold_right orb false (map (has_use (rel + #|defs|) ∘ dbody) defs)
+  | _ => false
+  end.
+
+Fixpoint valid_dearg_mask (mask : bitmask) (body : term) : Prop :=
+  match body, mask with
+  | tLetIn na val body, _ => valid_dearg_mask mask body
+  | tLambda _ body, b :: mask =>
+    (if b then has_use 0 body = false else True) /\ valid_dearg_mask mask body
+  | _, [] => True
+  | _, _ => False
+  end.
+
+Lemma dearg_cst_body_top_nil t :
+  dearg_cst_body_top [] t = t.
+Proof.
+  induction t; auto.
+  cbn.
+  now rewrite IHt2.
+Qed.
+
+Lemma dearg_single_0_mask mask args t :
+  Forall (eq false) mask ->
+  #|args| = #|mask| ->
+  dearg_single mask t args = mkApps t args.
+Proof.
+  intros mask_zero.
+  revert args t.
+  induction mask_zero.
+  - destruct args; easy.
+  - intros [|a args] t len_eq; [easy|].
+    subst.
+    cbn in *.
+    now apply IHmask_zero.
+Qed.
+
+Lemma dearg_single_snoc mask b t args a :
+  #|mask| = #|args| ->
+  dearg_single (mask ++ [b]) t (args ++ [a]) =
+  if b then
+    dearg_single mask t args
+  else
+    tApp (dearg_single mask t args) a.
+Proof.
+  revert t args b a.
+  induction mask as [|b mask IH]; intros t args bend aend len_eq.
+  - now destruct args as [|a args]; [|easy].
+  - destruct args as [|a args]; [easy|].
+    cbn in *.
+    destruct b.
+    + now apply IH.
+    + now apply IH.
+Qed.
+
+(* We introduce a concept of contexts much like PCUIC, except they are in the opposite
+   order; i.e. declarations are consed to the beginning *)
+Definition mkLambda_or_LetIn (cd : context_decl) (t : term) : term :=
+  match decl_body cd with
+  | None => tLambda (decl_name cd) t
+  | Some body => tLetIn (decl_name cd) body t
+  end.
+
+Definition it_mkLambda_or_LetIn (Γ : context) (t : term) : term :=
+  fold_right mkLambda_or_LetIn t Γ.
+
+Fixpoint decompose_body_masked (mask : bitmask) (t : term) : context * term :=
+  match mask, t with
+  | _, tLetIn na val body =>
+    let (Γ, t) := decompose_body_masked mask body in
+    (vdef na val :: Γ, t)
+  | b :: mask, tLambda na body =>
+    let (Γ, t) := decompose_body_masked mask body in
+    (vass na :: Γ, t)
+  | _, _ => ([], t)
+  end.
+
+Definition vasses (Γ : context) : context :=
+  filter (fun cd => match decl_body cd with
+                    | Some _ => false
+                    | None => true
+                    end) Γ.
+
+Lemma vasses_app Γ Γ' :
+  vasses (Γ ++ Γ') = vasses Γ ++ vasses Γ'.
+Proof.
+  unfold vasses.
+  now rewrite filter_app.
+Qed.
+
+Ltac refold :=
+  repeat
+    match goal with
+    | [H: context[fold_right _ ?t ?Γ] |- _] => progress (fold (it_mkLambda_or_LetIn Γ t) in * )
+    | [|- context[fold_right _ ?t ?Γ]] => progress (fold (it_mkLambda_or_LetIn Γ t) in * )
+    | [H: context[filter _ ?Γ] |- _] => progress (fold (vasses Γ) in * )
+    | [|- context[filter _ ?Γ]] => progress (fold (vasses Γ) in * )
+    end.
+
+Lemma decompose_body_masked_spec mask Γ t t' :
+  valid_dearg_mask mask t ->
+  (Γ, t') = decompose_body_masked mask t ->
+  #|vasses Γ| = #|mask| /\
+  it_mkLambda_or_LetIn Γ t' = t.
+Proof.
+  revert Γ t' mask.
+  induction t using term_forall_list_ind; intros Γ t' mask valid_mask eq.
+  all: cbn in *.
+  all: try solve [destruct mask; [|easy]; inversion eq; easy].
+  - destruct mask as [|b mask]; inversion eq; subst; clear eq; [easy|].
+    cbn in *.
+    destruct (decompose_body_masked mask t) as (Γ' & t'') eqn:decomp_eq.
+    inversion H0; subst; clear H0.
+    symmetry in decomp_eq.
+    cbn.
+    refold.
+    now destruct (IHt _ _ _ (proj2 valid_mask) decomp_eq) as (-> & ->).
+  - destruct (decompose_body_masked mask t2) eqn:decomp_eq.
+    symmetry in decomp_eq.
+    destruct (IHt2 _ _ _ valid_mask decomp_eq).
+    now destruct mask; inversion eq; subst.
+Qed.
+
+Lemma valid_dearg_mask_spec mask t :
+  valid_dearg_mask mask t ->
+  exists Γ inner,
+    #|vasses Γ| = #|mask| /\ it_mkLambda_or_LetIn Γ inner = t.
+Proof.
+  intros is_valid.
+  destruct (decompose_body_masked mask t) as (Γ & inner) eqn:decomp.
+  exists Γ, inner.
+  now apply decompose_body_masked_spec.
+Qed.
+
+(*
+Lemma valid_dearg_mask_inv mask body :
+  valid_dearg_mask mask body ->
+  exists Γ inner_body, body = it_mkLambda_or_LetIn Γ inner_body.
+Proof.
+  revert mask.
+  induction body using term_forall_list_ind; intros mask valid_mask; cbn in *.
+  - now exists [], tBox.
+  -
+
+Lemma valid_dearg_mask_snoc_inv mask body :
+  valid_dearg_mask (mask ++ [true]) body ->
+  exists context na inner_body,
+    body = it_mkLambda_or_LetIn context (tLambda na inner_body) /\
+    has_use 0 inner_body = false /\
+    valid_dearg_mask mask (it_mkLambda_or_LetIn context inner_body).
+Proof.
+  revert mask.
+  assert (H: forall mask,
+             match mask ++ [true] with
+             | [] => Forall (eq false) (mask ++ [true])
+             | b :: bs => Forall (eq false) (mask ++ [true])
+             end -> False).
+  { intros mask H.
+    destruct mask; cbn in *.
+    - inversion H; congruence.
+    - rewrite app_comm_cons in H.
+      apply Forall_app in H.
+      destruct H as [_ H].
+      now inversion H. }
+
+  induction body using term_forall_list_ind;
+    intros mask valid_mask; cbn in *; try solve [exfalso; easy]; clear H.
+  - destruct mask as [|b mask]; cbn in *.
+    + exists [], n, body.
+      easy.
+    +
+      destruct valid_mask as (use & valid_mask).
+      specialize (IHbody _ valid_mask).
+      destruct IHbody as (Γ & na & inner_body & -> & inner_unused & valid_it).
+      destruct b.
+      * exists (Γ ++ [vass n]), na, inner_body.
+        cbn.
+        cbn.
+        cbn.
+  intros is_valid.
+  Admitted.
+Lemma dearg_cst_body_top_snoc_true mask body :
+  valid_dearg_mask (mask ++ [true]) body ->
+  exists na Γ inner,
+    body = it_mkLambda_or_LetIn (Γ,, vass na) inner /\
+    dearg_cst_body_top (mask ++ [true]) body = it_mkLambda_or_LetIn Γ inner.
+Proof.
+  revert mask.
+  assert (H: forall mask,
+             match mask ++ [true] with
+             | [] => Forall (eq false) (mask ++ [true])
+             | b :: bs => Forall (eq false) (mask ++ [true])
+             end -> False).
+  { intros mask H.
+    destruct mask; cbn in *.
+    - inversion H; congruence.
+    - rewrite app_comm_cons in H.
+      apply Forall_app in H.
+      destruct H as [_ H].
+      now inversion H. }
+
+  induction body using term_forall_list_ind;
+    intros mask valid_mask; cbn in *; try solve [exfalso; easy]; clear H.
+  - admit.
+  - admit.
+Admitted.
+*)
+
+Fixpoint subst_context_aux (Γ : context) (inner : term) (args : list term) : term :=
+  match Γ with
+  | cd :: Γ =>
+    match decl_body cd with
+    | Some val => subst_context_aux Γ (csubst val 0 inner) args
+    | None =>
+      match args with
+      | a :: args => subst_context_aux Γ (csubst a 0 inner) args
+      | [] => inner
+      end
+    end
+  | [] => inner
+  end.
+
+Definition subst_context (Γ : context) (inner : term) (args : list term) : term :=
+  subst_context_aux (List.rev Γ) inner args.
+
+Lemma subst_context_aux_app Γ Γ' inner args :
+  #|vasses Γ| <= #|args| ->
+  subst_context_aux (Γ ++ Γ') inner args =
+  subst_context_aux Γ' (subst_context_aux Γ inner args) (skipn #|vasses Γ| args).
+Proof.
+  revert Γ' inner args.
+  induction Γ; intros Γ' inner args le.
+  - cbn.
+    now rewrite skipn_0.
+  - cbn in *.
+    refold.
+    destruct (decl_body a).
+    + easy.
+    + destruct args; cbn in *; [abstract lia|].
+      apply IHΓ.
+      abstract lia.
+Qed.
+
+Lemma filter_rev {A} f (l : list A) :
+  filter f (List.rev l) = List.rev (filter f l).
+Proof.
+  induction l; [easy|].
+  cbn.
+  rewrite filter_app.
+  cbn.
+  destruct (f a); cbn.
+  - now f_equal.
+  - now rewrite app_nil_r.
+Qed.
+
+Lemma vasses_rev Γ : vasses (List.rev Γ) = List.rev (vasses Γ).
+Proof. apply filter_rev. Qed.
+
+Lemma subst_context_app Γ Γ' inner args :
+  #|vasses Γ'| <= #|args| ->
+  subst_context (Γ ++ Γ') inner args =
+  subst_context Γ (subst_context Γ' inner args) (skipn #|vasses Γ'| args).
+Proof.
+  intros len.
+  unfold subst_context.
+  rewrite List.rev_app_distr.
+  rewrite subst_context_aux_app.
+  - now rewrite vasses_rev, List.rev_length.
+  - now rewrite vasses_rev, List.rev_length.
+Qed.
+
+Lemma subst_context_aux_enough_args Γ inner args :
+  subst_context_aux Γ inner args =
+  subst_context_aux Γ inner (firstn #|vasses Γ| args).
+Proof.
+  revert inner args.
+  induction Γ; intros inner args; [easy|].
+  cbn.
+  refold.
+  destruct (decl_body a).
+  - easy.
+  - destruct args; [easy|].
+    apply IHΓ.
+Qed.
+
+Lemma subst_context_enough_args Γ inner args :
+  subst_context Γ inner args =
+  subst_context Γ inner (firstn #|vasses Γ| args).
+Proof.
+  unfold subst_context.
+  replace #|vasses Γ| with #|vasses (List.rev Γ)|.
+  - apply subst_context_aux_enough_args.
+  - now rewrite vasses_rev, List.rev_length.
+Qed.
+
+Lemma firstn_all_app_eq {A} n (l l' : list A) :
+  n = #|l| ->
+  firstn n (l ++ l') = l.
+Proof.
+  intros ->.
+  replace #|l| with (#|l| + 0) by lia.
+  rewrite firstn_app_2.
+  cbn.
+  apply app_nil_r.
+Qed.
+
+Derive Signature for eval.
+Derive NoConfusionHom for term.
+
+Lemma eval_LetIn Σ na val body res :
+  Σ ⊢ tLetIn na val body ▷ res ->
+  exists val_res,
+    Σ ⊢ val ▷ val_res /\
+    Σ ⊢ csubst val_res 0 body ▷ res.
+Proof.
+  intros ev.
+  depind ev; try easy.
+  - destruct args using List.rev_ind; [easy|].
+    rewrite mkApps_app in *.
+    cbn in *.
+    congruence.
+  - destruct args using List.rev_ind.
+    + cbn in *.
+      depelim H.
+      subst f.
+      now eapply IHev.
+    + rewrite mkApps_app in *.
+      cbn in *.
+      congruence.
+Qed.
+
+Lemma eval_tApp_arg Σ hd arg res :
+  Σ ⊢ tApp hd arg ▷ res ->
+  exists arg_res,
+    Σ ⊢ arg ▷ arg_res.
+Proof.
+  intros ev.
+  depind ev; try easy.
+  - destruct args using List.rev_ind; [easy|].
+    destruct args' using List.rev_ind.
+    + unfold ETyping.is_constructor_or_box in *.
+      now rewrite nth_error_nil in H0.
+    + rewrite mkApps_app in *.
+      cbn in *.
+      exists x0.
+      apply Forall2_app_r in H2.
+      destruct H2.
+      congruence.
+  - destruct args using List.rev_ind.
+    + cbn in *.
+      subst f.
+      easy.
+    + rewrite mkApps_app in *.
+      cbn in *.
+      destruct args' using List.rev_ind.
+      * depelim H.
+        apply (f_equal (@List.length term)) in H.
+        rewrite app_length in H.
+        now cbn in H.
+      * apply Forall2_app_r in H.
+        exists x0.
+        destruct H.
+        congruence.
+Qed.
+
+(*
+Lemma eval_App Σ na body arg res :
+  Σ ⊢ tApp (tLambda na body) arg ▷ res ->
+  exists arg_res,
+    Σ ⊢ arg  ▷ arg_res /\
+    Σ ⊢ csubst arg_res 0 body ▷ res.
+Proof.
+  intros ev.
+  depind ev.
+  - depelim ev1.
+    + destruct args using List.rev_ind; [easy|].
+      rewrite mkApps_app in *.
+      cbn in *.
+      congruence.
+    + destruct args' using List.rev_ind; [easy|].
+      rewrite mkApps_app in *.
+      cbn in *.
+      congruence.
+  - exists a'.
+    split; [easy|].
+    depelim ev1.
+    + admit.
+    + admit.
+    + easy.
+  - SearchAbout mkApps.
+    pose proof (mkApps_elim f args).
+    rewrite <- H3 in H4.
+    cbn in H4.
+    depelim H4.
+    destruct n.
+    + rewrite skipn_0 in H1, H2.
+      cbn in *.
+      admit.
+    + rewrite skipn_S, skipn_nil in H1.
+      easy.
+  - admit.
+  - apply eval_to_value in ev1.
+    depelim ev1.
+    + unfold atom in H.
+    exists a'.
+    split; [easy|].
+    SearchAbout eval.
+    rewrite mkApps_nested in H3.
+    cbn in *.
+    inversion H4.
+    change (tApp (tLambda na body) arg) with (mkApps (tLambda na body) [arg]) in H3.
+    apply mkApps_eq_inj in H3; try easy.
+    2: {
+*)
+
+(*
+Lemma eval_mkApps_subst_context Σ Γ inner args res :
+  #|args| = #|vasses Γ| ->
+  Σ ⊢ mkApps (it_mkLambda_or_LetIn Γ inner) args ▷ res ->
+  Σ ⊢ subst_context Γ inner (List.rev args) ▷ res.
+Proof.
+  revert inner args res.
+  induction Γ as [|cd Γ IH] using List.rev_ind; intros inner args res len_eq ev.
+  - cbn in *.
+    now destruct args.
+  - rewrite vasses_app, app_length in len_eq; cbn in *.
+    destruct (decl_body cd) eqn:decl_eq.
+    + cbn in *.
+      rewrite subst_context_app by (abstract (rewrite List.rev_length; lia)).
+      rewrite it_mkLambda_or_LetIn_app in *.
+      cbn in *.
+      unfold mkLambda_or_LetIn in *.
+      rewrite decl_eq in *.
+      assert (exists args_res, Forall2 (eval Σ) args args_res) by admit.
+      assert (exists let_in_res,
+                 Σ ⊢ tLetIn (decl_name cd) t (it_mkLambda_or_LetIn Γ inner) ▷ let_in_res)
+        by admit.
+      destruct H0 as (let_in_res & eval_let_in).
+      apply eval_LetIn in eval_let_in.
+      destruct eval_let_in as (val_res & eval_t & eval_subst).
+Lemma eval_csubst_congr t tn b res :
+  Σ ⊢ t ▷ tn ->
+  Σ ⊢ csubst tn 0 b ▷ res ->
+  Σ ⊢ csubst t 0 b ▷ res.
+
+      epose proof (IH inner args _ ltac:(abstract lia)).
+      eapply eval_LetIn.
+    destruct args as [|a args] using List.rev_ind.
+    + cbn in *.
+*)
+
+(*
+Lemma eval_mkApps_it_mkLambda_or_LetIn Σ Γ inner args res :
+  #|args| = #|vasses Γ| ->
+  Σ ⊢ subst_context Γ inner (List.rev args) ▷ res ->
+  Σ ⊢ mkApps (it_mkLambda_or_LetIn Γ inner) args ▷ res.
+Proof.
+  revert inner args res.
+  induction Γ as [|cd Γ IH] using List.rev_ind; intros inner args res len_eq eval_res.
+  - cbn in *.
+    now destruct args.
+  - rewrite it_mkLambda_or_LetIn_app.
+    unfold vasses in len_eq; rewrite filter_app in len_eq; refold.
+    rewrite app_length in len_eq.
+    rewrite subst_context_app in eval_res by (abstract (rewrite List.rev_length; lia)).
+    cbn in *.
+    unfold mkLambda_or_LetIn.
+    destruct (decl_body cd) as [body|].
+    +
+    + destruct args as [|a args]; [cbn in *; abstract lia|].
+      cbn in *.
+      rewrite skipn_all_app_eq in eval_res by (abstract (rewrite List.rev_length; lia)).
+      rewrite subst_context_enough_args in eval_res.
+      rewrite firstn_all_app_eq in eval_res by (abstract (rewrite List.rev_length; lia)).
+      admit.
+Admitted.
+*)
+
+Fixpoint unlift_let_values (n k : nat)  (Γ : context) : context :=
+  match Γ with
+  | [] => []
+  | cd :: Γ =>
+    {| decl_name := decl_name cd; decl_body := option_map (unlift n k) (decl_body cd) |}
+       :: unlift_let_values n (S k) Γ
+  end.
+
+Fixpoint deass_context (mask : bitmask) (Γ : context) : context :=
+  match Γ with
+  | [] => []
+  | cd :: Γ =>
+    match decl_body cd with
+    | Some val => cd :: deass_context mask Γ
+    | None =>
+      match mask with
+      | true :: mask => unlift_let_values 1 0 (deass_context mask Γ)
+      | false :: mask => cd :: deass_context mask Γ
+      | [] => []
+      end
+    end
+  end.
+
+(*
+Lemma deass_context_app mask Γ Γ' :
+  #|vasses Γ| = #|mask| ->
+  deass_context mask (Γ ++ Γ') =
+  deass_context mask Γ ++ deass_context (skipn #|vasses Γ| mask) Γ'.
+Proof.
+  revert mask Γ'.
+  induction Γ as [|cd Γ IH]; intros mask Γ' len_le.
+  - cbn.
+    destruct mask; easy.
+  - cbn in *.
+    destruct (decl_body cd).
+    + cbn.
+      refold.
+      now f_equal.
+    + cbn.
+      refold.
+      destruct mask as [|b mask]; [cbn in *; abstract lia|].
+      destruct b.
+      *
+        rewrite <- plus_Snm_nSm.
+        apply IH.
+        cbn in *.
+        abstract lia.
+      * cbn in *.
+        unfold skipn; fold (skipn #|vasses Γ| mask). (* wtf *)
+        f_equal.
+        now apply IH.
+Qed.
+*)
+
+Lemma deass_context_enough mask Γ :
+  deass_context mask Γ = deass_context (firstn #|vasses Γ| mask) Γ.
+Proof.
+  revert mask.
+  induction Γ; intros mask; [easy|].
+  cbn.
+  destruct (decl_body a).
+  - f_equal.
+    easy.
+  - refold.
+    destruct mask as [|b mask]; [easy|].
+    destruct b; cbn; [easy|].
+    now f_equal.
+Qed.
+
+Lemma unlift_lift n k t :
+  unlift n k (lift n k t) = t.
+Proof.
+  revert k.
+  induction t using term_forall_list_ind; intros k; cbn in *; try easy.
+  - destruct (Nat.leb_spec k n0); cbn.
+    + destruct (Nat.leb_spec k (n + n0)); [|lia].
+      f_equal.
+      lia.
+    + now destruct (Nat.leb_spec k n0); [lia|].
+  - f_equal.
+    induction H; cbn; easy.
+  - f_equal; [easy|].
+    induction X; cbn; [easy|].
+    destruct x.
+    cbn.
+    rewrite IHX.
+    cbn in *.
+    easy.
+  - f_equal.
+    rewrite map_length.
+    revert k.
+    induction H; cbn; [easy|]; intros k.
+    replace (S (#|l| + k)) with (#|l| + S k) by lia.
+    f_equal.
+    + destruct x.
+      unfold map_def.
+      cbn in *.
+      f_equal.
+      easy.
+    + easy.
+  - f_equal.
+    rewrite map_length.
+    revert k.
+    induction H; cbn; [easy|]; intros k.
+    replace (S (#|l| + k)) with (#|l| + S k) by lia.
+    f_equal.
+    + destruct x.
+      unfold map_def.
+      cbn in *.
+      f_equal.
+      easy.
+    + easy.
+Qed.
+
+Lemma unlift_0 k t : unlift 0 k t = t.
+Proof.
+  rewrite <- (lift0_id t k).
+  rewrite unlift_lift.
+  now rewrite lift0_id.
+Qed.
+
+Lemma unlift_unlift n k n' k' t :
+  k + n' <= k' ->
+  k' <= k ->
+  unlift n k (unlift n' k' t) = unlift (n + n') k' t.
+Proof.
+  revert n k n' k'.
+  induction t using term_forall_list_ind; intros n' k n'' k' l1 l2; try easy;
+    cbn in *.
+  - repeat
+      (cbn;
+       match goal with
+       | [|- context[?a <=? ?b]] => destruct (Nat.leb_spec a b)
+       end);
+      try lia; try (f_equal; lia).
+  - f_equal.
+    rewrite map_map.
+    solve_all.
+  - f_equal.
+    solve_all.
+  - f_equal; solve_all.
+  - f_equal; solve_all.
+  - rewrite map_map, compose_on_snd.
+    f_equal; solve_all.
+  - f_equal; solve_all.
+  - rewrite map_map, map_length, ELiftSubst.compose_map_def.
+    f_equal; solve_all.
+  - rewrite map_map, map_length, ELiftSubst.compose_map_def.
+    f_equal; solve_all.
+Qed.
+
+Lemma permute_unlift n k n' k' t :
+  n' <= k' ->
+  k' <= k ->
+  unlift n k (unlift n' k' t) = unlift n' k' (unlift n (k+k') t).
+Proof.
+  revert n k n' k'.
+  induction t using term_forall_list_ind; intros n' k n'' k'' le1 le2; try easy;
+    cbn in *.
+  - repeat
+      (match goal with
+       | [|- context[?a <=? ?b]] => destruct (Nat.leb_spec a b)
+       end;
+       cbn);
+      try lia; try (f_equal; lia).
+    f_equal.
+
+Lemma unlift_1 n k t :
+  unlift n k (unlift 1 0 t) = unlift 1 0 (unlift n (k+1) t).
+Proof.
+  revert n k.
+  induction t using term_forall_list_ind; intros n' k; try easy;
+    cbn in *.
+  - repeat
+      (match goal with
+       | [|- context[?a <=? ?b]] => destruct (Nat.leb_spec a b)
+       end;
+       cbn);
+      try lia; try (f_equal; lia).
+  - f_equal.
+    rewrite !map_map.
+    solve_all.
+  - f_equal.
+    solve_all.
+  - f_equal; solve_all.
+  - f_equal; solve_all.
+  - rewrite map_map, compose_on_snd.
+    f_equal; solve_all.
+  - f_equal; solve_all.
+  - rewrite map_map, map_length, ELiftSubst.compose_map_def.
+    f_equal; solve_all.
+  - rewrite map_map, map_length, ELiftSubst.compose_map_def.
+    f_equal; solve_all.
+Qed.
+
+Lemma permute_unlift n k n' k' t :
+  k <= k' ->
+  unlift n k (unlift n' k' t) = unlift n' (k + k') (unlift n k t).
+Proof.
+  revert n k n' k'.
+  induction t using term_forall_list_ind; intros n' k n'' k' le; try easy;
+    cbn in *.
+  - repeat
+      (cbn;
+       match goal with
+       | [|- context[?a <=? ?b]] => destruct (Nat.leb_spec a b)
+       end);
+      try lia; try (f_equal; lia).
+*)
+
+Lemma dearg_cst_body_top_it_mkLambda_or_LetIn mask Γ inner n k :
+  #|vasses Γ| = #|mask| ->
+  unlift n k (dearg_cst_body_top mask (it_mkLambda_or_LetIn Γ inner)) =
+  it_mkLambda_or_LetIn
+    (unlift_let_values n k (deass_context mask Γ))
+    (unlift (#|filter id mask| + n) (#|Γ| + k) inner).
+Proof.
+  revert inner mask n k.
+  induction Γ as [|cd Γ IH]; intros inner mask n k len_eq.
+  - destruct mask; [|easy].
+    cbn.
+    now rewrite dearg_cst_body_top_nil.
+  - cbn in *; refold.
+    unfold mkLambda_or_LetIn.
+    destruct (decl_body cd) eqn:body_eq.
+    + cbn.
+      refold.
+      unfold mkLambda_or_LetIn.
+      rewrite body_eq.
+      cbn.
+      f_equal.
+      replace (S (#|Γ| + k)) with (#|Γ| + S k) by abstract lia.
+      now apply IH.
+    + cbn in *.
+      destruct mask as [|b mask]; [cbn in *; abstract lia|].
+      cbn in *.
+      destruct b; cbn.
+      *
+
+        rewrite IH by easy.
+        rewrite unlift_unlift.
+        SearchAbout (lift _ _ (lift _ _ _)).
+        rewrite IH by easy.
+        rewrite IH by easy.
+
+      * cbn.
+        unfold mkLambda_or_LetIn.
+        rewrite body_eq.
+        f_equal.
+        rewrite deass_context_enough.
+        rewrite firstn_all_app_eq by (rewrite List.rev_length; abstract lia).
+        now apply IHΓ.
+Admitted.
+
+Lemma dearg_single_correct mask body args Σ t :
+  Σ ⊢ mkApps body args ▷ t ->
+  valid_dearg_mask mask body ->
+  length args = length mask ->
+  Σ ⊢ dearg_single mask (dearg_cst_body_top mask body) args ▷ t.
+Proof.
+  intros eval valid_mask len_eq.
+  destruct (valid_dearg_mask_spec _ _ valid_mask) as (Γ & inner & Γlen & ->).
+  revert mask args t inner valid_mask eval len_eq Γlen.
+  induction Γ as [|cd Γ IH] using List.rev_ind; intros mask args t inner valid_mask ev len_eq Γlen.
+  - cbn in *.
+    destruct mask; [|easy].
+    destruct args; [|easy].
+    cbn.
+    now rewrite dearg_cst_body_top_nil.
+  - rewrite vasses_app, app_length in Γlen.
+    rewrite it_mkLambda_or_LetIn_app in *.
+    cbn in *.
+    unfold mkLambda_or_LetIn in *.
+    destruct (decl_body cd) eqn:decl_eq.
+    + cbn in *.
+      admit.
+    + cbn in *.
+      destruct mask as [|b mask]; [easy|].
+      destruct args as [|a args]; [easy|].
+      destruct b.
+      * cbn.
+      cbn.
+
+
+Lemma foo :
+  #|mask| = #|args| ->
+  Σ ⊢ dearg_single mask  args ▷ res
+
+Inductive eval_apps Σ res : term -> list term -> Prop :=
+| eval_apps_nil t : Σ ⊢ t ▷ res -> eval_apps_nil Σ res t []
+| eval_apps_cons t args :
+    eval_apps Σ res t args ->
+    Σ ⊢ tApp t
+
+Fixpoint mkApps_eval_spine :
+  -> mkApps t
+
+
+      Σ ⊢ mkApps hd args ▷ res
+  apply eval_mkApps_subst_context in eval; [|congruence].
+
+  induction Γ.
+  - cbn in *.
+    destruct mask; [|easy].
+    destruct args; [|easy].
+    now rewrite dearg_cst_body_top_nil.
+  - cbn in *; refold.
+
+
+    rewrite <- it_mkLambda_or_LetIn_unfold in *.
+  revert mask body t.
+  induction args as [|a args IH] using List.rev_ind; intros mask body t eval valid_mask len_eq.
+  - destruct mask as [|b mask]; [|easy].
+    now rewrite dearg_cst_body_top_nil.
+  - rewrite mkApps_app.
+    rewrite app_length in len_eq.
+    destruct mask as [|b mask] using List.rev_ind.
+    + rewrite dearg_cst_body_top_nil.
+      cbn.
+      now rewrite Prelim.emkApps_snoc.
+    + clear IHmask.
+      rewrite app_length in len_eq.
+      rewrite dearg_single_snoc by (cbn in *; abstract lia).
+      destruct b.
+      * destruct (dearg_cst_body_top_snoc_true mask body valid_mask)
+          as (na & Γ & inner & -> & ->).
+
+        destruct (valid_dearg_mask_snoc_true mask body valid_mask)
+          as (na & inner_body & -> & no_use & valid_inner & ->).
+        apply IH; [|easy|cbn in *; abstract lia].
+      admit.
+      unfold dearg_single.
+      intros
+    inversion eval; subst; clear eval.
+    +
+      destruct b.
+      *
+  intros eval valid_mask.
+  revert args t eval mask valid_mask.
+  induction body using term_forall_list_ind; intros args t eval mask valid_mask len_eq;
+    try solve [
+          cbn in *;
+          destruct mask as [|[] ?];
+          now rewrite ?dearg_single_0_mask].
+  - cbn in *.
+    clear IHbody.
+    revert mask valid_mask len_eq.
+    induction args as [|a args IH]; cbn in *; intros mask valid_mask len_eq.
+    + destruct mask; easy.
+    + destruct mask as [|b mask]; [easy|].
+      destruct b; cbn in *.
+      *
+    admit.
+  - cbn in *.
+    induction mask as [|b mask]; [easy|].
+    destruct args as [|a args]; [easy|].
+    destruct b; cbn in *.
+    + (* Arg was removed, use the fact that there is no use to show that unlift
+         commutes with beta application in this case. *)
+
+    destruct mask as [|[] ?].
+    + cbn in *.
+
+  - cbn in *.
+    destruct mask as [|[] ?].
+    + easy.
+    + now rewrite dearg_single_0_mask by easy.
+    + now rewrite dearg_single_0_mask by easy.
+  - cbn in *.
+    assert (Forall (eq false) mask).
+    { destruct mask as [|[] ?]; auto. }
+    rewrite dearg_single_0_mask by easy.
+
+  - cbn in *.
+    destruct mask; [|easy].
+    cbn.
+    now rewrite dearg_cst_body_top_nil.
+  - destruct mask as [|b mask]; [easy|].
+    cbn in *.
+    destruct b.
+    + induction body using term_forall_list_ind;
+        try solve [cbn in *; inversion_clear valid_mask; congruence].
+      * cbn in *.
+        inversion_clear valid_mask; try congruence.
+      * cbn in *.
+        inversion_clear valid_mask.
+
+Definition const_mask_wf_top Σ (p : kername * bitmask) : Prop :=
+  exists cst,
+    declared_constant Σ p.1 cst /\
+    match cst_body cst with
+    | Some body => valid_dearg_mask p.2 body
+    | None => False
+    end.
+
+Definition const_masks_wf_top Σ : Prop :=
+  Forall (const_mask_wf_top Σ) const_masks.
+
+Fixpoint enough_lambdas (mask : bitmask) (body : term) : Prop :=
+  match mask, body with
+  | _ :: mask, tLambda _ body => enough_lambdas mask body
+  | mask, _ => Forall (eq false) mask
+  end.
+
+Definition case_shape
+           (ind : inductive) (npars : nat)
+           (brs : list (nat * term)) : Prop :=
+  match get_mib_masks ind_masks (inductive_mind ind) with
+  | Some mib_masks =>
+    npars = length (param_mask mib_masks) /\
+    ∥ Alli (fun c '(_, br) =>
+            match find (fun '(ind', c', _) => (ind' =? inductive_ind ind) && (c' =? c))
+                       (ctor_masks mib_masks) with
+            | Some (_, _, mask) => enough_lambdas mask br
+            | None => True
+            end)
+         0 brs ∥
+  | None => True
+  end.
+
+(* Proposition representing that all case branches have the correct shapes
+   (iterated lambdas) to be dearged. *)
+Fixpoint case_shapes (t : term) : Prop :=
+  match t with
+  | tBox => True
+  | tRel _ => True
+  | tVar _ => True
+  | tEvar _ ts => fold_right and True (map case_shapes ts)
+  | tLambda _ body => case_shapes body
+  | tLetIn _ val body => case_shapes val /\ case_shapes body
+  | tApp hd arg => case_shapes arg /\ case_shapes hd
+  | tConst kn => True
+  | tConstruct ind c => True
+  | tCase (ind, npars) discr brs => case_shape ind npars brs /\
+                                    fold_right and True (map (case_shapes ∘ snd) brs)
+  | tProj p t => case_shapes t
+  | tFix defs _
+  | tCoFix defs _ => fold_right and True (map (case_shapes ∘ dbody) defs)
+  end.
+
+Notation dearg_ctor := (dearg_ctor ind_masks).
+Notation dearg_consts := (dearg_const const_masks).
+Notation dearg_case := (dearg_case ind_masks).
+Notation dearg_aux := (dearg_aux ind_masks const_masks).
+Notation dearg := (dearg ind_masks const_masks).
+Notation dearg_cst := (dearg_cst ind_masks const_masks).
+Notation dearg_mib := (dearg_mib ind_masks).
+Notation dearg_decl := (dearg_decl ind_masks const_masks).
+Notation dearg_env := (dearg_env ind_masks const_masks).
+
+Theorem dearg_env_eval Σ s t :
+  trans Σ ⊢ s ▷ t ->
+  const_masks_wf_top Σ ->
+  trans (dearg_env Σ) ⊢ dearg s ▷ dearg t.
+Proof.
